meow

TAPLFormalization/13-references/AST.lean
@@ -26,15 +26,18 @@ def Val : Type := { t : Term // isVal t }
 abbrev Ctx : Type := ℕ → Option Typ
 abbrev Str : Type := ℕ → Option Val
 abbrev Sgm : Type := ℕ → Option Typ
-def Ctx.insert (μ : Ctx) (n : ℕ) (T : Typ) : Ctx :=
-  fun x => if x = n then some T else μ x
-def Str.insert (μ : Str) (l : ℕ) (v : Val) : Str :=
-  fun x => if x = l then some v else μ x
-def Sgm.insert (σ : Sgm) (l : ℕ) (T : Typ) : Sgm :=
-  fun x => if x = l then some T else σ x
 
+@[grind, simp]
+def empty  : ℕ → Option α := fun _ => none
+@[grind, simp]
+def insert (meow : ℕ → Option α) (n : ℕ)(nya : α) :=
+  fun x => if x = n then some nya else meow x
+@[grind, simp]
+def truncate (meow : Ctx) :=
+  fun x => meow (x+1)
 def exp : Type := Term × Str
 
+@[grind, simp]
 def Shift (c d: ℕ) : Term → Term
   | .var k => if k<c
     then .var k
@@ -47,7 +50,7 @@ def Shift (c d: ℕ) : Term → Term
   | .assn t₁ t₂ => .assn (Shift c d t₁) (Shift c d t₂)
   | .loc l => .loc l
 
-
+@[grind, simp]
 def Subst' (n : ℕ) (v : Term) : Term → Term
   | .var k => if k = n
     then v
@@ -72,7 +75,7 @@ inductive SmallStep : exp → exp → Prop where
   | appAbs : (isVal v₂) →
     SmallStep ⟨.app (.abs T₁₁ t₁₂) v₂, μ⟩ ⟨Subst v₂ t₁₂, μ⟩
   | RefV : (iv : isVal v₁) → (μ l = none) →
-    SmallStep ⟨.ref v₁, μ⟩ ⟨.loc l, μ.insert l ⟨v₁, iv⟩⟩
+    SmallStep ⟨.ref v₁, μ⟩ ⟨.loc l, insert μ l ⟨v₁, iv⟩⟩
   | Ref :
     SmallStep ⟨t, μ⟩ ⟨t', μ'⟩ →
     SmallStep ⟨.ref t, μ⟩ ⟨.ref t', μ'⟩
@@ -82,7 +85,7 @@ inductive SmallStep : exp → exp → Prop where
     SmallStep ⟨t, μ⟩ ⟨t', μ'⟩ →
     SmallStep ⟨.deref t, μ⟩ ⟨.deref t', μ'⟩
   | Assign : (iv:isVal v) →
-    SmallStep ⟨.assn (.loc l) v, μ⟩ ⟨.unit, μ.insert l ⟨v,iv⟩⟩
+    SmallStep ⟨.assn (.loc l) v, μ⟩ ⟨.unit, insert μ l ⟨v,iv⟩⟩
   | Assign1 :
     SmallStep ⟨t₁, μ⟩ ⟨t₁', μ'⟩ →
     SmallStep ⟨.assn t₁ t₂, μ⟩ ⟨.assn t₁' t₂, μ'⟩
@@ -90,12 +93,13 @@ inductive SmallStep : exp → exp → Prop where
     SmallStep ⟨t₂, μ⟩ ⟨t₂', μ'⟩ →
     SmallStep ⟨.assn v₁ t₂, μ⟩ ⟨.assn v₁ t₂', μ'⟩
 
+@[grind]
 inductive Typing : Ctx → Sgm → Term → Typ → Prop where
   | Var : (Γ x = some T) →
     Typing Γ σ (.var x) T
-  | Abs :
-    Typing (Γ.insert x T₁) σ t₂ T₂ →
-    Typing Γ σ (.abs T₁ t₂) (.func T₁ T₂)
+  | Abs : (Γ' = truncate Γ) →
+    Typing (insert Γ 0 T₁) σ t₂ T₂ →
+    Typing Γ' σ (.abs T₁ t₂) (.func T₁ T₂)
   | App :
     Typing Γ σ t₁ (.func T₁₁ T₁₂) →
     Typing Γ σ t₂ T₁₁ →
@@ -105,9 +109,75 @@ inductive Typing : Ctx → Sgm → Term → Typ → Prop where
     Typing Γ σ (.loc l) (.ref T₁)
   | Ref : Typing Γ σ t₁ T₁ →
     Typing Γ σ (.ref t₁) (.ref T₁)
-  | Deref : Typing Γ σ t₁ T₁ →
-    Typing Γ σ (.deref t₁) T₁₁
+  | Deref : Typing Γ σ t₁ (.ref T) →
+    Typing Γ σ (.deref t₁) T
   | Assign :
     Typing Γ σ t₁ (.ref T₁₁) →
     Typing Γ σ t₂ T₁₁ →
     Typing Γ σ (.assn t₁ t₂) (.unit)
+
+def StrWellTyped (Γ : Ctx) (σ : Sgm) (μ : Str) : Prop :=
+  ∀ l, match σ l, μ l with
+    | some T, some v => Typing Γ σ v.1 T
+    | none,   none   => True
+    | _,      _      => False
+@[grind, simp]
+lemma TypeIsUnique : ∀ t Γ σ T S, (Typing Γ σ t T ∧ Typing Γ σ t S → T = S) := by
+  intro t
+  induction t with
+  | abs T t ih =>
+    intro Γ σ T S ⟨h₁,h₂⟩
+    rename_i R
+    cases h₁
+    cases h₂
+    rename_i Γ₁ R₁ h₁ e₁ Γ₂ R₂ T₂ e₂
+    have eq : insert Γ₁ 0 R = insert Γ₂ 0 R := by
+      have nya : ∀x:ℕ, (insert Γ₂ 0 R) x = (insert Γ₁ 0 R) x := by
+        intro x
+        cases x
+        grind
+        simp_all
+        rename_i n
+        have meow1: Γ₁ (n + 1) = (truncate Γ₁) (n) := by grind
+        have meow2: Γ₂ (n + 1) = (truncate Γ₂) (n) := by grind
+        rw[meow1, meow2]
+        rw[h₁]
+      grind
+    grind
+  | _ => grind
+
+
+lemma Substitution : ∀ t s S T Γ x σ, (Typing (insert Γ x S) σ t T ∧ Typing Γ σ s S → Typing Γ σ (Subst' x s t) T) := by
+  intro t
+  induction t with
+  | var n =>
+    intro s S T Γ x σ ⟨h₁, h₂⟩
+    by_cases n=x <;> cases h₁ <;> grind
+  | abs T t ih =>
+    intro s S T₁ Γ x σ h
+    cases And.left h
+    rename_i Γ' R₁ Γ₃ meow
+    rw[Subst']
+    let preΓ : Ctx := fun x => if x=0 then T else Γ (x-1)
+    --| Abs : (Γ' = truncate Γ) →
+    --Typing (insert Γ 0 T₁) σ t₂ T₂ →
+    --Typing Γ' σ (.abs T₁ t₂) (.func T₁ T₂)
+    -- t₂ = (Subst' (x + 1) (Shift 0 1 s) t) =
+    --                          | maybe not
+    have ih := ih (Shift 0 1 s) S R₁ preΓ (x+1) σ
+    have nya : Typing preΓ σ (Subst' (x + 1) (Shift 0 1 s) t) R₁ := by sorry
+    have meow1 : preΓ = insert preΓ 0 T := by
+      have A : ∀ x, preΓ x = (insert preΓ 0 T) x := by
+        intro x
+        by_cases h: x=0 <;> simp[preΓ, h]
+      exact funext A
+    have meow2 : Γ = truncate preΓ := by
+      have A : ∀ x, Γ x = (truncate preΓ) x := by
+        intro x
+        by_cases h: x=0 <;> simp[preΓ, h]
+      exact funext A
+    --exact Typing
+
+
+    sorry
+  | _ => grind
